theories/CTyping.v
@@ -1,0 +1,145 @@
+From Coq Require Import Utf8 List.
+From GhostTT.autosubst Require Import CCAST unscoped.
+From GhostTT Require Import BasicAST SubstNotations ContextDecl CScoping.
+
+Import ListNotations.
+
+Set Default Goal Selector "!".
+
+Open Scope subst_scope.
+
+Notation "A ⇒[ mx ] B" :=
+  (cPi mx A (shift ⋅ B))
+  (at level 20, mx at next level, right associativity).
+
+Reserved Notation "Γ ⊢ᶜ t : A"
+  (at level 80, t, A at next level, format "Γ  ⊢ᶜ  t  :  A").
+
+Reserved Notation "Γ ⊢ᶜ u ≡ v"
+  (at level 80, u, v at next level, format "Γ  ⊢ᶜ  u  ≡  v").
+
+Inductive conversion (Γ : ccontext) : cterm → cterm → Prop :=
+
+(** Computation rules **)
+
+| cconv_beta :
+    ∀ mx A t u,
+      Γ ⊢ᶜ capp (clam mx A t) u ≡ t <[ u .. ]
+
+(** Congruence rules **)
+
+(** A rule to quotient away all levels of Prop, making it impredicative **)
+| ccong_Prop :
+    ∀ i j,
+      Γ ⊢ᶜ cSort cProp i ≡ cSort cProp j
+
+| ccong_Pi :
+    ∀ mx A A' B B',
+      Γ ⊢ᶜ A ≡ A' →
+      (mx, A) :: Γ ⊢ᶜ B ≡ B' →
+      Γ ⊢ᶜ cPi mx A B ≡ cPi mx A' B'
+
+| ccong_clam :
+    ∀ mx A A' t t',
+      Γ ⊢ᶜ A ≡ A' →
+      (mx, A) :: Γ ⊢ᶜ t ≡ t' →
+      Γ ⊢ᶜ clam mx A t ≡ clam mx A' t'
+
+| ccong_app :
+    ∀ u u' v v',
+      Γ ⊢ᶜ u ≡ u' →
+      Γ ⊢ᶜ v ≡ v' →
+      Γ ⊢ᶜ capp u v ≡ capp u' v'
+
+(* Maybe not needed? *)
+| ccong_bot_elim :
+    ∀ m A A' p p',
+      Γ ⊢ᶜ A ≡ A' →
+      (* Needed because syntactically we don't know p and p' are irrelevant *)
+      Γ ⊢ᶜ p ≡ p' →
+      Γ ⊢ᶜ cbot_elim m A p ≡ cbot_elim m A' p'
+
+(** Structural rules **)
+
+| cconv_refl :
+    ∀ u,
+      Γ ⊢ᶜ u ≡ u
+
+| cconv_sym :
+    ∀ u v,
+      Γ ⊢ᶜ u ≡ v →
+      Γ ⊢ᶜ v ≡ u
+
+| cconv_trans :
+    ∀ u v w,
+      Γ ⊢ᶜ u ≡ v →
+      Γ ⊢ᶜ v ≡ w →
+      Γ ⊢ᶜ u ≡ w
+
+(** Proof irrelevance **)
+
+| cconv_irr :
+    ∀ p q,
+      ccxscoping Γ p cProp →
+      ccxscoping Γ q cProp →
+      Γ ⊢ᶜ p ≡ q
+
+where "Γ ⊢ᶜ u ≡ v" := (conversion Γ u v).
+
+Inductive ctyping (Γ : ccontext) : cterm → cterm → Prop :=
+
+| ctype_var :
+    ∀ x m A,
+      nth_error Γ x = Some (m, A) →
+      Γ ⊢ᶜ cvar x : (plus (S x)) ⋅ A
+
+| ctype_sort :
+    ∀ m i,
+      Γ ⊢ᶜ cSort m i : cSort cType (S i)
+
+| ctype_pi :
+    ∀ i j m mx A B,
+      Γ ⊢ᶜ A : cSort mx i →
+      (mx, A) :: Γ ⊢ᶜ B : cSort m j →
+      Γ ⊢ᶜ cPi mx A B : cSort m (max i j)
+
+| ctype_clam :
+    ∀ mx m i j A B t,
+      Γ ⊢ᶜ A : cSort mx i →
+      (mx, A) :: Γ ⊢ᶜ B : cSort m j →
+      (mx, A) :: Γ ⊢ᶜ t : B →
+      Γ ⊢ᶜ clam mx A t : cPi mx A B
+
+| ctype_app :
+    ∀ mx A B t u,
+      Γ ⊢ᶜ t : cPi mx A B →
+      Γ ⊢ᶜ u : A →
+      Γ ⊢ᶜ capp t u : B <[ u .. ]
+
+| ctype_bot :
+    Γ ⊢ᶜ cbot : cSort cProp 0
+
+| ctype_bot_elim :
+    ∀ i m A p,
+      Γ ⊢ᶜ A : cSort m i →
+      Γ ⊢ᶜ p : cbot →
+      Γ ⊢ᶜ cbot_elim m A p : A
+
+| ctype_conv :
+    ∀ i m A B t,
+      Γ ⊢ᶜ t : A →
+      Γ ⊢ᶜ A ≡ B →
+      Γ ⊢ᶜ B : cSort m i →
+      Γ ⊢ᶜ t : B
+
+where "Γ ⊢ᶜ t : A" := (ctyping Γ t A).
+
+(** Context formation **)
+
+Inductive cwf : ccontext → Prop :=
+| cwf_nil : cwf nil
+| cwf_cons :
+    ∀ Γ m i A,
+      cwf Γ →
+      Γ ⊢ᶜ A : cSort m i →
+      cwf ((m, A) :: Γ).
